\documentclass{article}
\input{Algo1Macros}

\begin{document}

\section{Ejercicio 1}

\pred{esValido}{t : toroide}{\\
	(|t| \geq 3) \land \\
	(\forall i : \ent)(((0 \leq i < |t|) \implicaLuego (|t[i]| \leq 3)) \yLuego (|t[i]| = |t[0]|))
	\\ }

\section{Ejercicio 2}

\pred{toroideMuerto}{t : toroide}{\\
	(\forall i : \ent)((0 \leq i < |t|) \implicaLuego (\forall j : \ent) ((0 \leq j < |t[i]|) \implicaLuego (t[i][j] = False)))
	\\ }

\section{Ejercicio 3}

\pred{posicionesVivas}{t : toroide, vivas : \TLista{\ent \times \ent}}{\\ 
	(\forall i : \ent)((0 \leq i < |vivas|) \implicaLuego (t[vivas[i]_0][vivas[i]_1]) = \True) \land \\
	(\forall j : \ent)((0 \leq j < |t|) \implicaLuego ((\forall k : \ent)((0 \leq k < |t[j]) \implicaLuego \\
	(t[j][k] \implica (j,k) \in vivas))))
	\\}

\section{Ejercicio 4}

\subsection{Función principal}
\aux{densidadPoblacion}{t : toroide}{\float}{\\
	cantidadVivos(t) / cantidadPoblacion(t)}

\subsection{Funciones auxiliares}
\aux{cantidadVivos}{t : toroide}{\float}{\\
	\sum_{i=0}^{|t|-1}
	\sum_{j=0}^{|t[i]|-1}
	\IfThenElse{t[i][j]}{1}{0}}

\aux{cantidadPoblacion}{t : toroide}{\float}{\\ |t| \cdot |t[0]|}

\section{Ejercicio 5}

\subsection{Función principal}
\aux{cantVecinosVivos}{t : toroide, f : \ent , c : \ent}{\ent}{\\
	\sum_{i=0}^{|t|-1}
	\sum_{j=0}^{|t[i]|-1}
	\IfThenElse{(t[i][j] = \True) \land esVecino(t,i,j,f,c)}{1}{0}}

\subsection{Funciones auxiliares}
\aux{esVecino}{t : toroide, i,j,f,c : \ent}{\bool}{\\
	(i = (f+1 \ mod \ |t|) \lor i = (f-1 \ mod \ |t|)) \land \\
	(j = (c+1 \ mod \ |t[0]|) \lor j = (c-1 \ mod \ |t[0]|))}

\section{Ejercicio 6}

\pred{evolucionDePosiciones}{t : toroide, posicion : $\ent \times \ent$}{\\
	\IfThenElse{t[(posicion)_0][(posicion)_1] = \True \\}
	{2 \leq cantVecinosVivos(t, (posicion)_0, (posicion)_1) \leq 3\\}
	{cantVecinosVivos(t, (posicion)_0, (posicion)_1) = 3}
	\\}

\section{Ejercicio 7}

\pred{evolucionToroide}{t1 : toroide, t2 : toroide}{\\
	(|t1| = |t1|) \land (|t1[0]| = |t1[0]|) \land \\
	(\forall i : \ent)((0 \leq i < |t1|) \implicaLuego \\
	(\forall j : \ent)((0 \leq j < |t1[i]) \implicaLuego (t2[i][j] = evolucionDePosicion(t1, (i, j)))))
	\\}

\end{document}
